do 2. before: convert (IP OP : Z), framework works now. HMAC has an unnecessary roundtrip in mkArg from Z -> Byte -> Z, so factoring that out now

HMAC_spec_harvard_list.v
@@ -4,7 +4,7 @@ Set Implicit Arguments.
 Require Import List.
 Require Import Arith.
 
-Require Import HMAC_functional_prog.
+Require Import HMAC_functional_prog_Z.
 Require Import Integers.
 Require Import Coqlib.
 Require Import sha_padding_lemmas.
@@ -215,14 +215,14 @@ Section Example.
 
 
  Definition ip:Blist := concat (list_repeat 64 [false; true; false; false; true; false; true; true]).
- Definition IP:byte := Byte.repr 210.
+ Definition IP:Z := 210.
  Transparent Byte.repr. 
 
  Lemma ip_conv : convertByteBits [false; true; false; false; true; false; true; true] 210.
   eexists; eexists; eexists; eexists; eexists; eexists; eexists; eexists.
   split. reflexivity. simpl. reflexivity.
  Qed.
- Lemma ipcorrect: bytes_bits_lists ip (byte_to_64list IP).
+ Lemma ipcorrect: bytes_bits_lists ip (HMAC_SHA256.sixtyfour IP).
    unfold ip, IP. simpl. unfold byte_to_64list, HMAC_SHA256.sixtyfour. simpl.
    repeat constructor; try apply ip_conv.
   Qed. 
@@ -230,12 +230,12 @@ Section Example.
 Lemma ONE: convertByteBits [true; false; false; false; false; false; false; false] 1.
   repeat eexists. Qed.
 
-Lemma inner_fst_equiv_example : exists k (ip  : Blist) K (IP : byte), 
+Lemma inner_fst_equiv_example : exists k (ip  : Blist) K (IP : Z), 
                           ((length K) * 8)%nat = (c + p)%nat /\
                           Zlength K = Z.of_nat SHA256_.BlockSize /\
                           (* TODO: first implies this *)
                           bytes_bits_lists k K /\
-                          bytes_bits_lists ip (byte_to_64list IP) /\
+                          bytes_bits_lists ip (HMAC_SHA256.sixtyfour IP) /\
                           bytes_bits_lists (BLxor k ip) (map Byte.unsigned
        (HMAC_SHA256.mkArg (map Byte.repr (HMAC_SHA256.mkKey K)) IP)) .
 
@@ -264,7 +264,10 @@ Proof.
   intros.
   generalize dependent H. generalize dependent H0. intros H0 H1.
   unfold convertByteBits. unfold asZ.
+  Print Byte.Z_mod_modulus. Print Z.lxor.
+  SearchAbout Z.lxor.
   (* need to exhibit b16 ... b23 *)
+   
 
 Admitted.  
 
@@ -299,6 +302,7 @@ Proof.
       *
         apply xor_correspondence.
         apply H. apply H0.
+Qed.
 (*
 H : convertByteBits [b0; b1; b2; b3; b4; b5; b6; b7] byte 
 H0 : convertByteBits [b8; b9; b10; b11; b12; b13; b14; b15] byte0
@@ -310,10 +314,9 @@ H0 : convertByteBits [b8; b9; b10; b11; b12; b13; b14; b15] byte0
         (Z.lxor (Byte.Z_mod_modulus byte) (Byte.Z_mod_modulus byte0)))
 
 *)
-Admitted.
 
-
-Lemma inner_fst_equiv' : exists (ip  : Blist) (IP : byte), 
+(*
+Lemma inner_fst_equiv_ipbyte : exists (ip  : Blist) (IP : byte), 
                           bytes_bits_lists ip (byte_to_64list IP) /\
                       forall (k : Blist) (K : list Z),
                           ((length K) * 8)%nat = (c + p)%nat ->
@@ -338,9 +341,10 @@ Proof.
 Print HMAC_SHA256.mkArg.
    
 Admitted.
+*)
 
 Lemma inner_fst_equiv_ipZ : exists (ip  : Blist) (IP : Z), 
-                          bytes_bits_lists ip (Z_to_64list IP) /\
+                          bytes_bits_lists ip (HMAC_SHA256.sixtyfour IP) /\
                       forall (k : Blist) (K : list Z),
                           ((length K) * 8)%nat = (c + p)%nat ->
                           Zlength K = Z.of_nat SHA256_.BlockSize ->
@@ -354,17 +358,16 @@ Proof.
   apply ipcorrect.
   intros. 
   unfold HMAC_SHA256.mkArg, HMAC_SHA256.mkArgZ, HMAC_SHA256.mkKey.
+  Opaque HMAC_SHA256.sixtyfour.
    simpl. rewrite H0. simpl. unfold HMAC_SHA256.zeroPad.
    assert (KL: length K0 = 64%nat). admit.
    rewrite KL.  simpl.  rewrite app_nil_r.
-   unfold HMAC_SHA256.sixtyfour.
-   unfold HMAC_SHA256.Nlist.
+   apply inner_general_map.
 
-   apply inner_general_map.     (* :( *)
+   - apply ipcorrect.
+   - apply H1.
 
-(* TODO: trying to fix this problem -- change IP to be of type Z? or change inner_general_map? *)
-
-Admitted.
+Qed.
 
   
   
